implement cbor_map_get in Pulse

pulse/share/steel/examples/pulse/dice/cbor/CBOR.Pulse.fst
@@ -1,2 +1,279 @@
 module CBOR.Pulse
 include CBOR.Pulse.Extern
+open Pulse.Lib.Pervasives
+open Pulse.Lib.Stick
+
+module Cbor = CBOR.Spec
+
+noeq
+type cbor_map_get_t =
+| Found of cbor
+| NotFound
+
+let rec list_ghost_assoc
+  (#key: Type)
+  (#value: Type)
+  (k: key)
+  (m: list (key & value))
+: GTot (option value)
+  (decreases m)
+= match m with
+  | [] -> None
+  | (k', v') :: m' ->
+    if FStar.StrongExcludedMiddle.strong_excluded_middle (k == k')
+    then Some v'
+    else list_ghost_assoc k m'
+
+let cbor_map_get_post_not_found
+  (p: perm)
+  (vkey: Cbor.raw_data_item)
+  (vmap: Cbor.raw_data_item)
+  (map: cbor)
+: Tot vprop
+= raw_data_item_match p map vmap ** pure (
+    Cbor.Map? vmap /\
+    list_ghost_assoc vkey (Cbor.Map?.v vmap) == None
+  )
+
+let cbor_map_get_post_found
+  (p: perm)
+  (vkey: Cbor.raw_data_item)
+  (vmap: Cbor.raw_data_item)
+  (map: cbor)
+  (value: cbor)
+: Tot vprop
+= exists_ (fun vvalue ->
+    raw_data_item_match p value vvalue **
+    (raw_data_item_match p value vvalue @==> raw_data_item_match p map vmap) **
+    pure (
+      Cbor.Map? vmap /\
+      list_ghost_assoc vkey (Cbor.Map?.v vmap) == Some vvalue
+  ))
+
+let cbor_map_get_post
+  (p: perm)
+  (vkey: Cbor.raw_data_item)
+  (vmap: Cbor.raw_data_item)
+  (map: cbor)
+  (res: cbor_map_get_t)
+: Tot vprop
+= match res with
+  | NotFound -> cbor_map_get_post_not_found p vkey vmap map
+  | Found value -> cbor_map_get_post_found p vkey vmap map value
+
+let cbor_map_get_invariant
+  (pmap: perm)
+  (vkey: Ghost.erased Cbor.raw_data_item)
+  (vmap: Ghost.erased Cbor.raw_data_item)
+  (map: cbor)
+  (res: cbor_map_get_t)
+  (i: cbor_map_iterator_t)
+  (l: list (Cbor.raw_data_item & Cbor.raw_data_item))
+: Tot vprop
+= match res with
+  | Found value -> cbor_map_get_post_found pmap vkey vmap map value ** pure (
+      Cbor.Map? vmap /\
+      Some? (list_ghost_assoc (Ghost.reveal vkey) (Cbor.Map?.v vmap))
+    )
+  | NotFound ->
+    cbor_map_iterator_match pmap i l **
+    (cbor_map_iterator_match pmap i l @==> raw_data_item_match pmap map vmap) **
+    pure (
+        Cbor.Map? vmap /\
+        list_ghost_assoc (Ghost.reveal vkey) (Cbor.Map?.v vmap) ==
+          list_ghost_assoc (Ghost.reveal vkey) l
+    )
+
+assume val elim_stick0
+  (_: unit)
+  (#hyp #concl: vprop)
+: stt_ghost unit emp_inames
+    ((hyp @==> concl) ** hyp)
+    (fun _ -> concl)
+
+assume val stick_refl0
+    (p: vprop)
+: stt_ghost unit emp_inames
+    (emp)
+    (fun _ -> p @==> p)
+
+
+```pulse
+ghost
+fn cbor_map_get_invariant_end
+  (pmap: perm)
+  (vkey: Ghost.erased Cbor.raw_data_item)
+  (vmap: Ghost.erased Cbor.raw_data_item)
+  (map: cbor)
+  (gres: Ghost.erased cbor_map_get_t)
+  (res: cbor_map_get_t)
+  (i: Ghost.erased cbor_map_iterator_t)
+  (l: Ghost.erased (list (Cbor.raw_data_item & Cbor.raw_data_item)))
+requires
+    cbor_map_get_invariant pmap vkey vmap map gres i l **
+    pure (
+        (Nil? l \/ Found? gres) /\
+        res == Ghost.reveal gres
+    )
+ensures
+    cbor_map_get_post pmap vkey vmap map res ** pure (
+      Cbor.Map? vmap /\
+      Found? res == Some? (list_ghost_assoc (Ghost.reveal vkey) (Cbor.Map?.v vmap))
+    )
+{
+    match res
+    {
+        NotFound ->
+        {
+            rewrite (cbor_map_get_invariant pmap vkey vmap map gres i l) // FIXME: WHY WHY WHY?
+                as (cbor_map_get_invariant pmap vkey vmap map NotFound i l);
+            unfold (cbor_map_get_invariant pmap vkey vmap map NotFound i l);
+            elim_stick0 ();
+            fold (cbor_map_get_post_not_found pmap vkey vmap map);
+            fold (cbor_map_get_post pmap vkey vmap map NotFound)
+        }
+        Found value ->
+        {
+            rewrite (cbor_map_get_invariant pmap vkey vmap map gres i l) // FIXME: WHY WHY WHY?
+                as (cbor_map_get_invariant pmap vkey vmap map (Found value) i l);
+            unfold (cbor_map_get_invariant pmap vkey vmap map (Found value) i l);
+            fold (cbor_map_get_post pmap vkey vmap map (Found value))
+        }
+    }
+}
+```
+assume
+val stick_consume_l
+    (_: unit)
+    (#p #q #r: vprop)
+: stt_ghost unit emp_inames
+    (p ** ((p ** q) @==> r))
+    (fun _ -> q @==> r)
+
+assume
+val stick_consume_r
+    (_: unit)
+    (#q #p #r: vprop)
+: stt_ghost unit emp_inames
+    (p ** ((q ** p) @==> r))
+    (fun _ -> q @==> r)
+
+assume
+val stick_trans
+    (_: unit)
+    (#p #q #r: vprop)
+: stt_ghost unit emp_inames
+    ((p @==> q) ** (q @==> r))
+    (fun _ -> p @==> r)
+
+assume
+val rewrite_with_implies
+    (p q: vprop)
+: stt_ghost unit emp_inames
+    (p ** pure (p == q))
+    (fun _ -> q ** (q @==> p))
+
+assume
+val stick_weaken_hyp_r
+    (hl hr #hr' #c: vprop)
+: stt_ghost unit emp_inames
+    ((hr' @==> hr) ** ((hl ** hr) @==> c))
+    (fun _ -> (hl ** hr') @==> c)
+
+assume
+val stick_weaken_hyp_l
+    (hl hr #hl' #c: vprop)
+: stt_ghost unit emp_inames
+    ((hl' @==> hl) ** ((hl ** hr) @==> c))
+    (fun _ -> (hl' ** hr) @==> c)
+
+```pulse
+fn cbor_map_get
+  (key: cbor)
+  (map: cbor)
+  (#pkey: perm)
+  (#pmap: perm)
+  (#vkey: Ghost.erased Cbor.raw_data_item)
+  (#vmap: Ghost.erased Cbor.raw_data_item)
+requires
+    (raw_data_item_match pkey key vkey ** raw_data_item_match pmap map vmap ** pure (
+      Cbor.Map? vmap /\
+      (~ (Cbor.Tagged? vkey \/ Cbor.Array? vkey \/ Cbor.Map? vkey))
+    ))
+returns res: cbor_map_get_t
+ensures
+    (raw_data_item_match pkey key vkey ** cbor_map_get_post pmap vkey vmap map res ** pure (
+      Cbor.Map? vmap /\
+      Found? res == Some? (list_ghost_assoc (Ghost.reveal vkey) (Cbor.Map?.v vmap))
+    ))
+{
+    let i0 = cbor_map_iterator_init map;
+    with l0 . assert (cbor_map_iterator_match pmap i0 l0);
+    let done0 = cbor_map_iterator_is_done i0;
+    let mut pi = i0;
+    let mut pres = NotFound;
+    let mut pdone = done0;
+    fold (cbor_map_get_invariant pmap vkey vmap map NotFound i0 l0);
+    while (
+        with gres i l . assert (pts_to pres gres ** pts_to pi i ** cbor_map_get_invariant pmap vkey vmap map gres i l);
+        let res = !pres;
+        let done = !pdone;
+        assert (pts_to pres gres ** cbor_map_get_invariant pmap vkey vmap map gres i l); // FIXME: WHY WHY WHY?
+        not (done || Found? res)
+    )
+    invariant cont . exists (done: bool) (res: cbor_map_get_t) (i: cbor_map_iterator_t) (l: list (Cbor.raw_data_item & Cbor.raw_data_item)) .
+        raw_data_item_match pkey key vkey ** 
+        pts_to pdone done **
+        pts_to pi i **
+        pts_to pres res **
+        cbor_map_get_invariant pmap vkey vmap map res i l **
+        pure (
+            done == Nil? l /\
+            cont == not (done || Found? res)
+        )
+    {
+        with gres gi l . assert (pts_to pres gres ** cbor_map_get_invariant pmap vkey vmap map gres gi l);
+        rewrite each gres as NotFound;
+        unfold (cbor_map_get_invariant pmap vkey vmap map NotFound gi l);
+        let x = cbor_map_iterator_next pi;
+        stick_trans ();
+        with gi' l'. assert (cbor_map_iterator_match pmap gi' l');
+        with vx . assert (raw_data_item_map_entry_match pmap x vx);
+        rewrite_with_implies
+            (raw_data_item_map_entry_match pmap x vx)
+            (raw_data_item_match pmap (cbor_map_entry_key x) (fstp vx) **
+                raw_data_item_match pmap (cbor_map_entry_value x) (sndp vx)
+            );
+        let test = cbor_is_equal key (cbor_map_entry_key x);
+        if (test) {
+            stick_consume_l ()
+                #(raw_data_item_match pmap (cbor_map_entry_key x) (fstp vx))
+                #(raw_data_item_match pmap (cbor_map_entry_value x) (sndp vx));
+            stick_weaken_hyp_l
+                (raw_data_item_map_entry_match pmap x vx)
+                (cbor_map_iterator_match pmap gi' l');
+            stick_consume_r ()
+                #(raw_data_item_match pmap (cbor_map_entry_value x) (sndp vx))
+                #(cbor_map_iterator_match pmap gi' l');
+            pres := Found (cbor_map_entry_value x);
+            fold (cbor_map_get_post_found pmap vkey vmap map (cbor_map_entry_value x));
+            fold (cbor_map_get_invariant pmap vkey vmap map (Found (cbor_map_entry_value x)) gi' l)
+        } else {
+            elim_stick0 ()
+                #(raw_data_item_match pmap (cbor_map_entry_key x) (fstp vx) ** raw_data_item_match pmap (cbor_map_entry_value x) (sndp vx));
+            stick_consume_l ()
+                #(raw_data_item_map_entry_match pmap x vx)
+                #(cbor_map_iterator_match pmap gi' l');
+            let i' = !pi;
+            rewrite each gi' as i';
+            let done = cbor_map_iterator_is_done i';
+            pdone := done;
+            fold (cbor_map_get_invariant pmap vkey vmap map NotFound i' l')
+        }
+    };
+    with gres i l . assert (pts_to pres gres ** cbor_map_get_invariant pmap vkey vmap map gres i l);
+    let res = !pres;
+    cbor_map_get_invariant_end pmap vkey vmap map gres res i l;
+    res
+}
+```
